src/lowparse/pulse/LowParse.Pulse.BitSum.fst
@@ -122,3 +122,36 @@ let read_bitsum'
         stt_cps_ifthenelse
         (read_bitsum'_cont b)
     )
+
+inline_for_extraction
+let pure_read_synth_cont_ifthenelse
+  (#t: Type0)
+  (x: Ghost.erased t)
+: Tot (if_combinator_weak (pure_read_synth_cont_t #t x))
+= fun cond iftrue iffalse t' g' -> if cond then iftrue () t' g' else iffalse () t' g'
+
+inline_for_extraction
+let pure_read_bitsum'
+  (#t: eqtype)
+  (#tot: pos)
+  (#cl: uint_t tot t)
+  (#b: bitsum' cl tot)
+  (d: destr_bitsum'_t b)
+  (#k: parser_kind)
+  (#p: parser k t)
+  (#s: serializer p)
+  (r: pure_reader s)
+: Tot (pure_reader (tot_serialize_bitsum' b s))
+= pure_read_synth
+    (pure_read_filter
+      r
+      (filter_bitsum' b)
+    )
+    (synth_bitsum'_injective b; synth_bitsum' b)
+    (synth_bitsum'_recip_inverse b; synth_bitsum'_recip b)
+    (
+      d
+        (pure_read_synth_cont_t #(bitsum'_type b))
+        (pure_read_synth_cont_ifthenelse #(bitsum'_type b))
+        (pure_read_synth_cont_init)
+    )
